Types, terms, values, substitution

Stlc.v
@@ -1,3 +1,125 @@
 Require Export Types.
 
+Module STLC.
+
+Inductive ty : Type :=
+| TBool : ty
+| TArrow : ty -> ty -> ty.
+
+Inductive tm : Type :=
+| tvar : id -> tm
+| tapp : tm -> tm -> tm
+| tabs : id -> ty -> tm -> tm
+| ttrue : tm
+| tfalse : tm
+| tif : tm -> tm -> tm -> tm.
+
+Tactic Notation "t_cases" tactic(first) ident(c) :=
+    first;
+    [ Case_aux c "tvar" | Case_aux c "tapp"
+    | Case_aux c "tabs" | Case_aux c "ttrue"
+    | Case_aux c "tfalse" | Case_aux c "tif" ].
+
+Definition x := (Id 0).
+Definition y := (Id 1).
+Definition z := (Id 2).
+Hint Unfold x.
+Hint Unfold y.
+Hint Unfold z.
+
+(* idB = \x:Bool . x *)
+Notation idB := (tabs x TBool (tvar x)).
+
+(* idBB = \x:(Bool -> Bool) . x *)
+Notation idBB := (tabs x (TArrow TBool TBool) (tvar x)).
+
+(* idBBB = \x:(Bool->Bool) -> (Bool -> Bool) . x *)
+Notation idBBBB := (tabs x (TArrow (TArrow TBool TBool)
+                                   (TArrow TBool TBool)) (tvar x)).
+(* k = \x:Bool . \y:Bool . x *)
+Notation k := (tabs x TBool (tabs y TBool (tvar))).
+
+(* notB = \x:Bool . if x then false else true *)
+Notation notB := (tabs x TBool (tif (tvar x) false true)).
+
+Inductive value : tm -> Prop :=
+| v_abs   : forall x T t, value (tabs x T t)
+| v_true  : value ttrue
+| v_false : value tfalse.
+
+Hint Constructors value.
+
+Reserved Notation "'[' x ':=' s ']' t" (at level 20).
+
+Fixpoint subst (x:id) (s:tm) (t:tm) : tm :=
+    match t with
+    | tvar x'      => if eq_id_dec x x' then s else t
+    | tabs x' T t1 =>
+          tabs x' T (if eq_id_dec x x' then t1 else ([x:=s] t1))
+    | tapp t1 t2   => tapp ([x:=s] t1) ([x:=s] t2)
+    | ttrue        => ttrue
+    | tfalse       => tfalse
+    | tif t1 t2 t3 =>
+          tif ([x:=s] t1) ([x:=s] t2) ([x:=s] t3)
+    end
+
+where "'[' x ':=' s ']' t" := (subst x s t).
+
+
+Inductive substi (s:tm) (x:id) : tm -> tm -> Prop :=
+| s_var1 : substi s x (tvar x) s
+| s_var2 : forall y, x <> y ->
+             substi s x (tvar y) (tvar y)
+| s_abs1 : forall T t1, substi s x (tabs x T t1) (tabs x T t1)
+| s_abs2 : forall y, x <> y ->
+           forall t1 t1', substi s x t1 t1' ->
+           forall T, substi s x (tabs y T t1) (tabs y T t1')
+| s_app  : forall t1 t1' t2 t2',
+           substi s x t1 t1' ->
+           substi s x t2 t2' ->
+           substi s x (tapp t1 t2) (tapp t1' t2')
+| s_ttrue : substi s x ttrue ttrue
+| s_tfalse : substi s x tfalse tfalse
+| s_tif : forall t1 t1' t2 t2' t3 t3',
+          substi s x t1 t1' ->
+          substi s x t2 t2' ->
+          substi s x t3 t3' ->
+          substi s x (tif t1 t2 t3) (tif t1' t2' t3').
+
+Hint Constructors substi.
+
+Theorem substi_correct : forall s x t t',
+    [x:=s]t = t' <-> substi s x t t'.
+Proof.
+    split.
+    Case "->".
+        generalize dependent t'.
+        t_cases (induction t) SCase;
+            simpl; intros;
+               (try (inversion H; clear H));
+               (try (destruct (eq_id_dec x0 i)); subst);
+               auto.
+    Case "<-".
+        intro H. induction H; simpl; auto.
+        SCase "s_var1".
+            auto using eq_id.
+        SCase "s_var2".
+            auto using neq_id.
+        SCase "s_abs1".
+            rewrite -> eq_id. reflexivity.
+        SCase "s_abs2".
+            rewrite -> neq_id.
+              rewrite -> IHsubsti. reflexivity.
+              assumption.
+        SCase "s_app".
+            rewrite -> IHsubsti1.
+            rewrite -> IHsubsti2.
+            reflexivity.
+        SCase "s_tif".
+            rewrite -> IHsubsti1.
+            rewrite -> IHsubsti2.
+            rewrite -> IHsubsti3.
+            reflexivity.
+Qed.
+
 
